WIP on transitivity

theories/lang/cpp/semantics/ptrs.v
@@ -368,6 +368,42 @@ Module Type PTRS_MIXIN (Import P : PTRS_INTF_MINIMAL).
         p1 = p ,, o1 /\
         p2 = p ,, o2 /\
         offset_cong σ o1 o2.
+
+  Section implicit_type_off.
+    (* TODO lift *)
+    Implicit Type (o : offset).
+
+    Axiom ptr_common_prefix : ∀ {p1 p2 o1 o2},
+      p1 ,, o1 = p2 ,, o2 ->
+      ∃ p oa ob,
+      p1 = p ,, oa /\ p2 = p ,, ob.
+    Definition add_opt (oz1 oz2 : option Z) : option Z :=
+      match oz1, oz2 with
+      | Some z1, Some z2 => Some (z1 + z2)
+      | _, _ => None
+      end.
+    (* Argh, not true!
+    TODO: strengthen
+    *)
+    #[global] Instance add_opt_inj : ∀ a, Inj eq eq (add_opt a).
+    Proof. Admitted.
+    Axiom eval_offset_dot : ∀ σ (o1 o2 : offset),
+      eval_offset σ (o1 ,, o2) =
+      add_opt (eval_offset σ o1) (eval_offset σ o2).
+    Axiom ptr_vaddr_dot : ∀ σ p o,
+      Z.of_N <$> ptr_vaddr (p ,, o) =
+      add_opt (Z.of_N <$> ptr_vaddr p) (eval_offset σ o).
+    Corollary ptr_vaddr_dot_derived {σ p o1 o2} :
+      ptr_vaddr (p ,, o1) = ptr_vaddr (p ,, o2) ->
+      eval_offset σ o1 = eval_offset σ o2.
+    Proof.
+      move=> /(f_equal (fmap (M := option) Z.of_N)).
+      rewrite !ptr_vaddr_dot.
+      apply: inj.
+    Qed.
+  End implicit_type_off.
+
+
   #[global] Instance ptr_cong_equivalence {σ : genv} : Equivalence (ptr_cong σ).
   Proof.
     constructor; red; unfold ptr_cong.
@@ -378,14 +414,21 @@ Module Type PTRS_MIXIN (Import P : PTRS_INTF_MINIMAL).
       exists p'', o2, o1; intuition done.
     - intros p p' p''
              [p''' [o1 [o2 [Hp [Hp' Hos]]]]]
-             [p'''' [o1' [o2' [Hp'' [Hp''' Hos']]]]];
-        subst.
-      do 3 eexists; intuition eauto.
-      rewrite Hp''.
-      (* Leibniz equality on [_dot p o = _dot p o'] doesn't seem to hold
-         when [offset_cong o o'] does
-       *)
-  Abort.
+             [p'''' [o1' [o2' [Hp'' [Hp''' Hos']]]]].
+      subst.
+      destruct (ptr_common_prefix Hp'') as (p0 & oa & ob & ? & ?); subst.
+      exists p0.
+      exists (oa ,, o1).
+      exists (ob ,, o2').
+      rewrite !offset_ptr_dot.
+      intuition.
+      move: Hos Hos'.
+      rewrite /offset_cong !eval_offset_dot => -> <-.
+      move: (Hp'').
+      rewrite -!offset_ptr_dot.
+      move=> /(f_equal ptr_vaddr) /ptr_vaddr_dot_derived.
+      by rewrite !eval_offset_dot.
+    Qed.
 
   (** ** [same_address] lemmas *)
 
